clightplus_examples/xorlist/xorlist01proof.v
@@ -1303,10 +1303,12 @@ Section PROOF.
   Theorem correct : refines2 [xor0; ClightPlusMem0.Mem] [xorlist1.xor xor0 GlobalStb; ClightPlusMem1.Mem].
   Proof.
     eapply adequacy_local_strong_l. econs; cycle 1.
-    { econs; ss. econs; ss. }
-    i. econs; ss; cycle 1.
-    { econs; ss. apply correct_mod; et. inv SKINCL. inv H6. ss. }
-    unfold _xor, compile, get_sk in VALID. des_ifs. ss.
+    { econs; [ss|]. econs; ss. }
+    i. econs; cycle 1.
+    { econs; [|ss]. apply correct_mod; et. inv SKINCL. inv H6. ss. }
+    unfold _xor, compile, get_sk in VALID.
+    destruct Pos.eq_dec; [|clarify].
+    destruct Coqlib.list_norepet_dec; ss. des_ifs_safe.
     econstructor 1 with (wf := wf) (le := top2); et; ss; cycle 1.
     { eexists. econs. apply to_semantic. iIntros. et. }
     (* each functions has simulation relation *)
